Prove closure conversion correct

src/named/SimpleClosureConv.v
@@ -6,109 +6,273 @@ Import ListNotations.
 Open Scope string.
 Open Scope list.
 From Utils Require Import Utils.
-From Named Require Import Core Compilers Elab ElabCompilers
-     SimpleVSubst SimpleVSTLC SimpleProd Matches.
+From Named Require Import Core Compilers Elab ElabCompilersWithPrefix
+     SimpleVSubst SimpleVSTLC SimpleProd Matches
+ CatProd.
 Import Core.Notations.
 (*TODO: repackage this in compilers*)
 Import CompilerDefs.Notations.
 
 Require Coq.derive.Derive.
 
+(*TODO: construct the right hierarchy on top of cat;
+  currently copy-pasted
+*)
+(*
+Depends on: (rename _ cat), catprod
+ob -> ty
+arr -> val
+
+expr extension
+*)
 Definition closure_lang :=
   [
-  [:> "G" : #"env",
+  [:> "G" : #"ty",
       "A" : #"ty",
       "B" : #"ty",
       "A_fvs" : #"ty",
-      "e" : #"el" (#"ext" #"emp" (#"prod" %"A_fvs" %"A")) %"B",
+      "e" : #"exp" (#"prod" %"A_fvs" %"A") %"B",
       "fvs" : #"val" %"G" %"A_fvs"
       ----------------------------------------------- ("ret_closure")
       (#"closure" %"A" %"e" (#"ret" %"fvs"))
       = #"ret" (#"closure_val" %"A" %"e" %"fvs")
-      : #"el" %"G" (#"clo" %"A" %"B")
+      : #"exp" %"G" (#"clo" %"A" %"B")
   ];
-  [:> "G" : #"env",
+  [:> "G" : #"ty",
       "A" : #"ty",
       "B" : #"ty",
       "A_fvs" : #"ty",
-      "e" : #"el" (#"ext" #"emp" (#"prod" %"A_fvs" %"A")) %"B",
+      "e" : #"exp" (#"prod" %"A_fvs" %"A") %"B",
       "fvs" : #"val" %"G" %"A_fvs",
-      "G'" : #"env",
-      "g" : #"sub" %"G'" %"G"
+      "G'" : #"ty",
+      "g" : #"val" %"G'" %"G"
       ----------------------------------------------- ("closure_val_subst")
       #"val_subst" %"g" (#"closure_val" %"A" %"e" %"fvs")
       = #"closure_val" %"A" %"e" (#"val_subst" %"g" %"fvs")
       : #"val" %"G'" (#"clo" %"A" %"B")
   ];
-  [:> "G" : #"env",
+  [:> "G" : #"ty",
       "A" : #"ty",
       "B" : #"ty",
       "A_fvs" : #"ty",
-      "e" : #"el" (#"ext" #"emp" (#"prod" %"A_fvs" %"A")) %"B",
-      "fvs" : #"el" %"G" %"A_fvs",
-      "G'" : #"env",
-      "g" : #"sub" %"G'" %"G"
+      "e" : #"exp" (#"prod" %"A_fvs" %"A") %"B",
+      "fvs" : #"exp" %"G" %"A_fvs",
+      "G'" : #"ty",
+      "g" : #"val" %"G'" %"G"
       ----------------------------------------------- ("closure_subst")
       #"el_subst" %"g" (#"closure" %"A" %"e" %"fvs")
       = #"closure" %"A" %"e" (#"el_subst" %"g" %"fvs")
-      : #"el" %"G'" (#"clo" %"A" %"B")
+      : #"exp" %"G'" (#"clo" %"A" %"B")
   ];
-  [:> "G" : #"env", "A" : #"ty", "B" : #"ty",
-      "e" : #"el"%"G" (#"clo" %"A" %"B"),
-      "e'" : #"el" %"G" %"A",
-      "G'" : #"env",
-      "g" : #"sub" %"G'" %"G"
+  [:> "G" : #"ty", "A" : #"ty", "B" : #"ty",
+      "e" : #"exp" %"G" (#"clo" %"A" %"B"),
+      "e'" : #"exp" %"G" %"A",
+      "G'" : #"ty",
+      "g" : #"val" %"G'" %"G"
       ----------------------------------------------- ("clo_app_subst")
       #"el_subst" %"g" (#"clo_app" %"e" %"e'")
       = #"clo_app" (#"el_subst" %"g" %"e") (#"el_subst" %"g" %"e'")
-      : #"el" %"G'" %"B"
+      : #"exp" %"G'" %"B"
   ];
-  [:> "G" : #"env",
+  [:> "G" : #"ty",
+      "A" : #"ty",
+      "B" : #"ty",
+      "v" : #"val" %"G" (#"clo" %"A" %"B")
+      ----------------------------------------------- ("clo_eta")
+      (#"closure_val" %"A"
+        (#"clo_app" (#"ret" (#"val_subst" #".1" %"v")) (#"ret" #".2"))
+        #"id")
+      = %"v"
+      : #"val" %"G" (#"clo" %"A" %"B")
+  ];
+  [:> "G" : #"ty",
       "A" : #"ty",
       "B" : #"ty",
       "A_fvs" : #"ty",
-      "e" : #"el" (#"ext" #"emp" (#"prod" %"A_fvs" %"A")) %"B",
+      "e" : #"exp" (#"prod" %"A_fvs" %"A") %"B",
       "fvs" : #"val" %"G" %"A_fvs",
       "v" : #"val" %"G" %"A"
       ----------------------------------------------- ("clo_beta")
       #"clo_app" (#"ret" (#"closure_val" %"A" %"e" %"fvs")) (#"ret" %"v")
-      = #"el_subst" (#"snoc" #"forget" (#"pair_val" %"fvs" %"v")) %"e"
-      : #"el" %"G" %"B"
+      = #"el_subst" (#"pair" %"fvs" %"v") %"e"
+      : #"exp" %"G" %"B"
   ];
-  [:| "G" : #"env",
+  [:| "G" : #"ty",
        "A" : #"ty",
        "B" : #"ty",
-       "e" : #"el" %"G" (#"clo" %"A" %"B"),
-       "e'" : #"el" %"G" %"A"
+       "e" : #"exp" %"G" (#"clo" %"A" %"B"),
+       "e'" : #"exp" %"G" %"A"
        -----------------------------------------------
-       #"clo_app" "e" "e'" : #"el" %"G" %"B"
+       #"clo_app" "e" "e'" : #"exp" %"G" %"B"
   ];
-  [:| "G" : #"env",
+  [:| "G" : #"ty",
        "A" : #"ty",
        "B" : #"ty",
        "A_fvs" : #"ty",
-       "e" : #"el" (#"ext" #"emp" (#"prod" %"A_fvs" %"A")) %"B",
+       "e" : #"exp" (#"prod" %"A_fvs" %"A") %"B",
        "fvs" : #"val" %"G" %"A_fvs"
        -----------------------------------------------
        #"closure_val" "A" "e" "fvs" : #"val" %"G" (#"clo" %"A" %"B")
   ];
     (* have an expression closure to evaluate fvs*)
-  [:| "G" : #"env",
+  [:| "G" : #"ty",
        "A" : #"ty",
        "B" : #"ty",
        "A_fvs" : #"ty",
-       "e" : #"el" (#"ext" #"emp" (#"prod" %"A_fvs" %"A")) %"B",
-       "fvs" : #"el" %"G" %"A_fvs"
+       "e" : #"exp" (#"prod" %"A_fvs" %"A") %"B",
+       "fvs" : #"exp" %"G" %"A_fvs"
        -----------------------------------------------
-       #"closure" "A" "e" "fvs" : #"el" %"G" (#"clo" %"A" %"B")
+       #"closure" "A" "e" "fvs" : #"exp" %"G" (#"clo" %"A" %"B")
   ];
   [:| "A" : #"ty", "B": #"ty"
       -----------------------------------------------
       #"clo" "A" "B" : #"ty"
-    ]]%arule.
+  ]]%arule
+    ++
+    (*****************************
+      TODO: move language below out into multiple 
+      dependencies
+
+     *********************************)
+    [[:> "G" : #"ty", "A" : #"ty"
+       ----------------------------------------------- ("pair_wkn_hd")
+        #"pair" #".1" #".2" = #"id" : #"val" (#"prod" %"G" %"A") (#"prod" %"G" %"A")
+   ];
+   [:> "G1" : #"ty", "G2" : #"ty", "G3" : #"ty",
+       "f" : #"val" %"G1" %"G2",
+       "g" : #"val" %"G2" %"G3",
+       "A" : #"ty",
+       "v" : #"val" %"G2" %"A"
+       ----------------------------------------------- ("val_subst_pair")
+       #"val_subst" %"f" (#"pair" %"g" %"v")
+       = #"pair" (#"val_subst" %"f" %"g") (#"val_subst" %"f" %"v")
+       : #"val" %"G1" (#"prod" %"G3" %"A")
+   ];
+   [:> "G" : #"ty", "G'" : #"ty",
+       "g" : #"val" %"G" %"G'",
+       "A" : #"ty",
+       "v" : #"val" %"G" %"A"
+       ----------------------------------------------- ("pair_hd")
+       #"val_subst" (#"pair" %"g" %"v") #".2" = %"v"
+       : #"val" %"G" %"A"
+  ];
+  [:> "G" : #"ty", "G'" : #"ty",
+      "g" : #"val" %"G" %"G'",
+      "A" : #"ty",
+      "v" : #"val" %"G" %"A"
+      ----------------------------------------------- ("wkn_pair")
+      #"val_subst" (#"pair" %"g" %"v") #".1" = %"g" : #"val" %"G" %"G'"
+  ];
+  [:| "G" : #"ty", "A" : #"ty"
+       -----------------------------------------------
+       #".2" : #"val" (#"prod" %"G" %"A") %"A"
+  ];
+  [:| "G" : #"ty", "A" : #"ty"
+       -----------------------------------------------
+       #".1" : #"val" (#"prod" %"G" %"A") %"G"
+  ];
+  [:| "G" : #"ty", "G'" : #"ty", "A" : #"ty",
+      "g" : #"val" %"G" %"G'",
+      "v" : #"val" %"G" %"A" (*we restrict substitutions to values *)
+       -----------------------------------------------
+       #"pair" "g" "v" : #"val" %"G" (#"prod" %"G'" %"A")
+  ];
+  [:| "G" : #"ty", "A": #"ty"
+       -----------------------------------------------
+       #"prod" "G" "A" : #"ty"
+  ];
+    (*TODO: generalize to all programs of type unit?*)
+  [:> 
+      ----------------------------------------------- ("id_emp_forget")
+      #"id" = #"forget" : #"val" #"unit" #"unit"
+  ];
+  [:> "G" : #"ty", "G'" : #"ty", "g" : #"val" %"G" %"G'"
+       ----------------------------------------------- ("val_subst_forget")
+       #"val_subst" %"g" #"forget" = #"forget" : #"val" %"G" #"unit"
+  ];
+  [:| "G" : #"ty" 
+      -----------------------------------------------
+      #"forget" : #"val" %"G" #"unit"
+  ];
+  [:| 
+      -----------------------------------------------
+      #"unit" : #"ty"
+  ];
+  [:> "G1" : #"ty", "G2" : #"ty",
+       "g" : #"val" %"G1" %"G2",
+       "A" : #"ty", "v" : #"val" %"G2" %"A"
+       ----------------------------------------------- ("el_subst_ret")
+       #"el_subst" %"g" (#"ret" %"v")
+       = #"ret" (#"val_subst" %"g" %"v")
+       : #"exp" %"G1" %"A"
+  ];
+  [:| "G" : #"ty", "A" : #"ty", "v" : #"val" %"G" %"A"
+       -----------------------------------------------
+       #"ret" "v" : #"exp" %"G" %"A"
+  ];
+  [:> "G1" : #"ty", "G2" : #"ty", "G3" : #"ty",
+       "f" : #"val" %"G1" %"G2", "g" : #"val" %"G2" %"G3",
+       "A" : #"ty", "e" : #"exp" %"G3" %"A"
+       ----------------------------------------------- ("el_subst_val_subst")
+       #"el_subst" %"f" (#"el_subst" %"g" %"e")
+       = #"el_subst" (#"val_subst" %"f" %"g") %"e"
+       : #"exp" %"G1" %"A"
+  ]; 
+  [:> "G" : #"ty", "A" : #"ty", "e" : #"exp" %"G" %"A"
+       ----------------------------------------------- ("el_subst_id")
+       #"el_subst" #"id" %"e" = %"e" : #"exp" %"G" %"A"
+  ]; 
+  [:| "G" : #"ty", "G'" : #"ty", "g" : #"val" %"G" %"G'",
+       "A" : #"ty", "e" : #"exp" %"G'" %"A"
+       -----------------------------------------------
+       #"el_subst" "g" "e" : #"exp" %"G" %"A"
+  ]; 
+  [s| "G" : #"ty", "A" : #"ty"
+      -----------------------------------------------
+      #"exp" "G" "A" srt
+  ];
+   [:> "G1" : #"ty",
+         "G2" : #"ty",
+         "G3" : #"ty",
+         "G4" : #"ty",
+         "f" : #"val" %"G1" %"G2",
+         "g" : #"val" %"G2" %"G3",
+         "h" : #"val"%"G3" %"G4"
+         ----------------------------------------------- ("val_subst_assoc")
+         #"val_subst" %"f" (#"val_subst" %"g" %"h")
+         = #"val_subst" (#"val_subst" %"f" %"g") %"h"
+         : #"val" %"G1" %"G4"
+  ];  
+  [:> "G" : #"ty", "G'" : #"ty", "f" : #"val" %"G" %"G'"
+       ----------------------------------------------- ("id_left")
+       #"val_subst" #"id" %"f" = %"f" : #"val" %"G"%"G'"
+  ];
+  [:> "G" : #"ty", "G'" : #"ty", "f" : #"val" %"G" %"G'"
+      ----------------------------------------------- ("id_right")
+      #"val_subst" %"f" #"id" = %"f" : #"val" %"G" %"G'"
+  ];
+  [:| "G1" : #"ty", "G2" : #"ty", "G3" : #"ty",
+       "f" : #"val" %"G1" %"G2",
+       "g" : #"val" %"G2" %"G3"
+       -----------------------------------------------
+       #"val_subst" "f" "g" : #"val" %"G1" %"G3"
+  ];
+  [:| "G" : #"ty" 
+       -----------------------------------------------
+       #"id" : #"val" %"G" %"G"
+  ];
+  [s| "G" : #"ty", "G'" : #"ty" 
+      -----------------------------------------------
+      #"val" "G" "G'" srt                     
+  ];
+  [s|
+      -----------------------------------------------
+      #"ty" srt
+   ]]%arule.
+
 
 Derive closure_elab
-       SuchThat (Pre.elab_lang (prod_elab ++ subst_elab) closure_lang closure_elab)
+       SuchThat (Pre.elab_lang [] closure_lang closure_elab)
        As closure_wf.
 Proof. auto_elab. Qed.
 #[export] Hint Resolve closure_wf : elab_pfs.
@@ -123,17 +287,19 @@ Definition cc : compiler :=
   | {{s #"env" }} => {{s #"ty"}}
   | {{s #"sub" "G" "G'"}} => {{s #"val" %"G" %"G'"}}
   | {{e #"id" "G"}} => {{e #"id"}}
-  | {{e #"cmp" "G1" "G2" "G3" "f" "g"}} => {{e #"cmp_val" %"f" %"g"}}
-  | {{s #"el" "G" "A"}} => {{s #"el" %"G" %"A" }}
-  | {{e #"el_subst" "G1" "G2" "f" "A" "e"}} => {{e #"cmp" %"f" %"e"}}
+  | {{e #"cmp" "G1" "G2" "G3" "f" "g"}} => {{e #"val_subst" %"f" %"g"}}
+  | {{s #"el" "G" "A"}} => {{s #"exp" %"G" %"A" }}
+  (*TODO: rename target to exp_subst*)
+  | {{e #"el_subst" "G1" "G2" "f" "A" "e"}} => {{e #"el_subst" %"f" %"e"}}
   | {{s #"val" "G" "A"}} => {{s #"val" %"G" %"A" }}
-  | {{e #"val_subst" "G1" "G2" "f" "A" "v"}} => {{e #"cmp_val" %"f" %"v"}}
+  | {{e #"val_subst" "G1" "G2" "f" "A" "v"}} => {{e #"val_subst" %"f" %"v"}}
   | {{e #"ret" "G" "A" "v" }} => {{e #"ret" %"v"}}
   | {{e #"ext" "G" "A"}} => {{e #"prod" %"G" %"A" }}
-  | {{e #"snoc" "G" "G'" "A" "g" "v"}} => {{e #"pair_val" %"g" %"v"}}
+  | {{e #"emp" }} => {{e #"unit"}}
+  | {{e #"snoc" "G" "G'" "A" "g" "v"}} => {{e #"pair" %"g" %"v"}}
   (*Note that we need complex values here to accommodate this projection *)
-  | {{e #"wkn" "G" "A"}} => {{e #".1_val" #"id" }}
-  | {{e #"hd" "G" "A"}} => {{e #".2_val" #"id" }}
+  | {{e #"wkn" "G" "A"}} => {{e #".1" }}
+  | {{e #"hd" "G" "A"}} => {{e #".2" }}
   | {{e #"->" "A" "B"}} => {{e #"clo" %"A" %"B" }}
   | {{e #"lambda" "G" "A" "B" "e"}} =>
     {{e #"closure_val" %"A" %"e" #"id"}}
@@ -141,51 +307,118 @@ Definition cc : compiler :=
     {{e #"clo_app" %"e" %"e'"}}
   end.
 
+(*TODO: move *)
 
-Derive cps_elab
-       SuchThat (elab_preserving_compiler stlc_bot cps cps_elab (nth_tail 1 stlc_bot))
-       As cps_elab_preserving.
+Inductive names_match (A B : Type) : named_list A -> named_list B -> Type :=
+    nm_nil : names_match [] []
+  | nm_cons : forall (a : A) (a' : B) l l' n,
+      names_match l l' -> names_match ((n,a) :: l) ((n,a') :: l').
+#[export] Hint Constructors names_match : lang_core.
+
+Lemma eq_term_by'_right name l c e1 e2 t c' e1' e2' t' s s'
+  : wf_lang l ->
+    In [:> ! c
+           ----------------------------------------------- (name)
+           {e1} = {e2} : {t}
+       ]%arule l ->
+    names_match c s ->
+    matches_unordered e2' e2 = Some s' ->
+    incl s' s ->
+    e2' = e2[/s/] ->
+    e1' = e1[/s/] ->
+    t' = t[/s/] ->
+    wf_subst l c' s c ->
+    eq_term l c' t' e1' e2'.
 Proof.
-  pose proof stlc_bot_wf.
- match goal with
-  | |- elab_preserving_compiler _ ?cmp ?ecmp ?src =>
-        rewrite (as_nth_tail cmp); rewrite (as_nth_tail ecmp); rewrite (as_nth_tail src)
- end.
-
-
- break_preserving.
-
- all: try solve[ repeat t; repeat t'].
- all: try solve [is_term_rule].
-
- solve[ compute_eq_compilation;by_reduction].
- solve[ compute_eq_compilation;by_reduction].
- solve[ compute_eq_compilation;by_reduction].
- apply cps_subst_preserved.
- apply cps_beta_preserved.
-
- solve[ compute_eq_compilation;by_reduction].
- Unshelve.
- compute in cps_elab.
- all: repeat t'.
+  intros; subst.
+  eapply eq_term_subst; [| eapply eq_subst_refl; eassumption | ..].
+  use_rule_in_wf; basic_core_crush.
+  basic_core_crush.
 Qed.
 
+Arguments eq_term_by'_right _ : clear implicits.
 
-Local Lemma stlc_wf' : wf_lang (nth_tail 1 stlc_bot).
+Derive cc_elab
+       SuchThat (elab_preserving_compiler [] closure_elab
+                                          cc cc_elab (stlc_elab ++ subst_elab))
+       As cc_elab_preserving.
 Proof.
-  change (nth_tail 1 stlc_bot) with (stlc_elab ++ subst_elab).
-  eauto 7 with auto_elab elab_pfs.
-Qed.
+  
+  (*TODO: replace the original with this*)
+  Ltac term_cong ::=
+  eapply term_con_congruence;
+   [ solve_in
+   | solve_len_eq
+   | compute; reflexivity
+   | eauto with elab_pfs auto_elab
+   | repeat
+      match goal with
+      | |- eq_args _ _ _ _ _ =>
+            simple apply eq_args_nil || simple eapply eq_args_cons2 || simple eapply eq_args_cons
+      end ].
 
-Goal semantics_preserving stlc_bot cps_elab (nth_tail 1 stlc_bot).
-Proof.
-  apply inductive_implies_semantic.
-  - apply stlc_wf'.
-  - apply stlc_bot_wf.
-  - eauto using cps_elab_preserving with lang_core.
-Qed.
+  setup_elab_compiler; repeat t.
+  solve [ compute_eq_compilation; by_reduction ].
+  solve [ compute_eq_compilation; by_reduction ].
+  solve [ compute_eq_compilation; by_reduction ].
+  solve [ compute_eq_compilation; by_reduction ].
+  solve [ compute_eq_compilation; by_reduction ].
+  solve [ compute_eq_compilation; by_reduction ].
+  solve [ compute_eq_compilation; by_reduction ].
+  solve [ compute_eq_compilation; by_reduction ].
+  solve [ compute_eq_compilation; by_reduction ].
+  solve [ compute_eq_compilation; by_reduction ].
+  solve [ compute_eq_compilation; by_reduction ].
+  solve [ compute_eq_compilation; by_reduction ].
+  solve [ compute_eq_compilation; by_reduction ].
+  solve [ compute_eq_compilation; by_reduction ].
+  solve [ compute_eq_compilation; by_reduction ].
+  solve [ compute_eq_compilation; by_reduction ].
 
-(*
-TODO: make proof generate fully evalled cps_elab to print w/ the notation
-Eval compute in cps_elab.
-*)
+  
+  compute_eq_compilation.
+  eapply eq_term_trans.
+  reduce.
+  eapply eq_term_sym.
+  eapply eq_term_trans.
+  reduce.
+  eapply eq_term_trans.
+  2:{
+    eapply (eq_term_by'_right "clo_eta").
+    eauto with auto_elab elab_pfs.
+    solve_in.
+    eauto with lang_core.
+    compute;reflexivity.
+    {
+      repeat (rewrite incl_cons).
+      intuition.
+    }
+    compute; reflexivity.
+    compute; reflexivity.
+    compute; reflexivity.
+    repeat apply wf_subst_cons.
+    constructor.
+    repeat t'.
+    repeat t'.
+    repeat t'.
+    repeat t'.
+  }
+  term_cong.
+  term_refl.
+  term_refl.
+  term_refl.
+  term_refl.
+  compute_eq_compilation.
+  {
+    eapply eq_term_sym.
+    eapply eq_term_trans.
+    reduce.
+    term_refl.
+  }
+  term_refl.
+   
+  Unshelve.
+  all: repeat t'; eauto
+   with elab_pfs auto_elab.
+Qed.
+#[export] Hint Resolve cc_elab_preserving : elab_pfs.
